src/TV/seop_llvmop.v
@@ -696,7 +696,7 @@ Case "dbIcmp".
 Case "dbSelect".
   inversion H; subst. clear H.
   exists l0. exists ps. exists cs. exists tmn0.
-  exists (if c then updateAddAL _ lc0 id0 gv1 else updateAddAL _ lc0 id0 gv2). exists als0. exists Mem1.
+  exists (if c then updateAddAL _ lc0 id0 gv2 else updateAddAL _ lc0 id0 gv1). exists als0. exists Mem1.
   exists cs1. split; auto.
   right. left.
   exists (insn_select id0 v0 t v1 v2).
