src/ssa/ssa_extract.v
@@ -1,0 +1,380 @@
+Add LoadPath "./ott".
+Add LoadPath "./monads".
+Add LoadPath "../../../theory/metatheory".
+
+Require Import ssa_dynamic.
+Require Import trace.
+Require Import Metatheory.
+Require Import assoclist.
+Require Import monad.
+Require Import genericvalues.
+Require Import ssa_mem.
+
+Export LLVMopsem.
+
+Definition interInsn (state:State) : option (State*trace) :=
+(* Check if the stack is empty. *) 
+match state with
+| mkState Sys TD Ps nil gl Mem0 => None
+| mkState Sys TD Ps ((mkEC F B cs tmn lc arg0 als)::EC) gl Mem0 =>
+  (* If cs is nil, we check tmn, 
+     otherwise, we check the first cmd in cs *)
+  match cs with
+  | nil => (* terminator *)
+    match tmn with
+    | insn_return rid RetTy Result =>
+      (* the suspended stacks cannot be empty, and
+          there must be a caller of the current function. *)
+      match EC with
+      | nil => None
+      | (mkEC F' B' nil tmn' lc' arg' als')::EC'' => None
+      | (mkEC F' B' (c'::cs') tmn' lc' arg' als')::EC'' =>
+        (* there must be a caller of the current function. *)
+        if (Instruction.isCallInst c') 
+        then 
+          do Mem' <- free_allocas Mem0 als;
+             ret ((mkState Sys TD Ps ((mkEC F' B' cs' tmn' (returnUpdateLocals TD c' RetTy Result lc lc' gl) arg' als')::EC'') gl Mem'),
+                  trace_nil)
+        else None
+      end
+    | insn_return_void rid =>
+      (* the suspended stacks cannot be empty, and
+          there must be a caller of the current function. *)
+      match EC with
+      | nil => None
+      | (mkEC F' B' nil tmn' lc' arg' als')::EC'' => None
+      | (mkEC F' B' (c'::cs') tmn' lc' arg' als')::EC'' =>
+        (* there must be a caller of the current function. *)
+        if (Instruction.isCallInst c')
+        then
+          do Mem' <- free_allocas Mem0 als;
+             ret ((mkState Sys TD Ps ((mkEC F' B' cs' tmn' lc' arg' als')::EC'') gl Mem'),
+                  trace_nil)
+        else None
+      end
+    | insn_br bid Cond l1 l2 =>
+      (* read the value of Cond *)
+      do cond0 <- (getOperandInt TD 1 Cond lc gl);
+      (* look up the target block *)
+        match (if (cond0:nat)
+               then lookupBlockViaLabelFromFdef F l1
+               else lookupBlockViaLabelFromFdef F l2) with
+        | None => None
+        | Some (block_intro l' ps' cs' tmn') =>
+            Some ((mkState Sys TD Ps ((mkEC F (block_intro l' ps' cs' tmn') cs' tmn' 
+                     (switchToNewBasicBlock (block_intro l' ps' cs' tmn') B lc) arg0 als)::EC) gl Mem0),
+                  trace_nil)
+        end
+    | insn_br_uncond bid l0 =>
+      (* look up the target block *)
+      match (lookupBlockViaLabelFromFdef F l0) with
+      | None => None
+      | Some (block_intro l' ps' cs' tmn') =>
+          Some ((mkState Sys TD Ps ((mkEC F (block_intro l' ps' cs' tmn') cs' tmn' 
+                        (switchToNewBasicBlock (block_intro l' ps' cs' tmn') B lc) arg0 als)::EC) gl Mem0),
+               trace_nil)
+      end
+    | insn_unreachable _ => None
+    end
+
+  | c::cs => (* non-terminator *)
+    match c with
+    | insn_bop id0 bop0 sz0 v1 v2 => 
+      do gv3 <- BOP TD lc gl bop0 sz0 v1 v2;
+         ret ((mkState Sys TD Ps ((mkEC F B cs tmn (updateAddAL _ lc id0 gv3) arg0 als)::EC) gl Mem0),
+              trace_nil)         
+    | insn_extractvalue id0 t v idxs =>
+      do gv <- getOperandValue TD v lc gl;
+      do gv' <- extractGenericValue TD t gv idxs;
+         ret ((mkState Sys TD Ps ((mkEC F B cs tmn (updateAddAL _ lc id0 gv') arg0 als)::EC) gl Mem0),
+              trace_nil)
+    | insn_insertvalue id0 t v t' v' idxs =>
+      do gv <- getOperandValue TD v lc gl;
+      do gv' <- getOperandValue TD v' lc gl;
+      do gv'' <- insertGenericValue TD t gv idxs t' gv';
+         ret ((mkState Sys TD Ps ((mkEC F B cs tmn (updateAddAL _ lc id0 gv'') arg0 als)::EC) gl Mem0),
+             trace_nil)
+    | insn_malloc id0 t sz0 align0 =>
+      do tsz <- getTypeAllocSize TD t;
+      match (malloc TD Mem0 (tsz * sz0) align0) with
+      | None => None
+      | Some (Mem', mb) =>
+        ret ((mkState Sys TD Ps ((mkEC F B cs tmn (updateAddAL _ lc id0 (ptr2GV TD (mb, 0))) arg0 als)::EC) gl Mem'),
+            trace_nil)
+      end
+    | insn_free fid t v =>
+      do mptr <- getOperandPtr TD v lc gl;
+      do Mem' <- free Mem0 mptr;
+         ret ((mkState Sys TD Ps ((mkEC F B cs tmn lc arg0 als)::EC) gl Mem'), trace_nil)
+    | insn_alloca id0 t sz0 align0 =>
+      do tsz <- getTypeAllocSize TD t;
+      match (malloc TD Mem0 (tsz * sz0) align0) with
+      | None => None
+      | Some (Mem', mb) =>
+          ret ((mkState Sys TD Ps ((mkEC F B cs tmn (updateAddAL _ lc id0 (ptr2GV TD (mb, 0))) arg0 (mb::als))::EC) gl Mem'),
+              trace_nil)
+      end
+    | insn_load id0 t v align0 =>
+      do mp <- getOperandPtr TD v lc gl;
+      do gv <- mload TD Mem0 mp t align0;
+         ret ((mkState Sys TD Ps ((mkEC F B cs tmn (updateAddAL _ lc id0 gv) arg0 als)::EC) gl Mem0),
+              trace_nil)
+    | insn_store sid t v1 v2 align0 =>
+      do gv1 <- getOperandValue TD v1 lc gl;
+      do mp2 <- getOperandPtr TD v2 lc gl;
+      do Mem' <- mstore TD Mem0 mp2 t gv1 align0;
+         ret ((mkState Sys TD Ps ((mkEC F B cs tmn lc arg0 als)::EC) gl Mem'),
+             trace_nil)
+    | insn_gep id0 inbounds0 t v idxs =>
+      do mp <- getOperandPtr TD v lc gl;
+      do mp' <- GEP TD lc gl t mp idxs inbounds0;
+         ret ((mkState Sys TD Ps ((mkEC F B cs tmn (updateAddAL _ lc id0 (ptr2GV TD mp')) arg0 als)::EC) gl Mem0),
+             trace_nil)
+    | insn_ext id0 extop0 t1 v1 t2 =>
+      do gv2 <- EXT TD lc gl extop0 t1 v1 t2;
+         ret ((mkState Sys TD Ps ((mkEC F B cs tmn (updateAddAL _ lc id0 gv2) arg0 als)::EC) gl Mem0),
+             trace_nil)
+    | insn_cast id0 castop0 t1 v1 t2 =>
+      do gv2 <- CAST TD lc gl castop0 t1 v1 t2;
+         ret ((mkState Sys TD Ps ((mkEC F B cs tmn (updateAddAL _ lc id0 gv2) arg0 als)::EC) gl Mem0),
+             trace_nil)
+    | insn_icmp id0 cond0 t v1 v2 =>
+      do gv3 <- ICMP TD lc gl cond0 t v1 v2;
+         ret ((mkState Sys TD Ps ((mkEC F B cs tmn (updateAddAL _ lc id0 gv3) arg0 als)::EC) gl Mem0),
+             trace_nil)
+    | insn_select id0 v0 t v1 v2 =>
+      do cond0 <- getOperandInt TD 1 v0 lc gl;
+      do gv1 <- getOperandValue TD v1 lc gl;
+      do gv2 <- getOperandValue TD v2 lc gl;
+         ret ((mkState Sys TD Ps ((mkEC F B cs tmn (if (cond0:nat) then updateAddAL _ lc id0 gv2 else updateAddAL _ lc id0 gv1) arg0 als)::EC) gl Mem0),
+             trace_nil)  
+    | insn_call rid noret0 tailc0 rt fid lp =>
+      (* only look up the current module for the time being, 
+         do not support linkage. *)
+      match (lookupFdefViaIDFromProducts Ps fid) with
+      | None => None
+      | Some (fdef_intro (fheader_intro rt' fid' la) lb) =>
+        if id_dec fid fid' then
+          if typ_dec rt rt' then
+            match (getEntryBlock (fdef_intro (fheader_intro rt fid la) lb)) with
+            | None => None
+            | Some (block_intro l' ps' cs' tmn') =>
+                ret ((mkState Sys TD Ps ((mkEC (fdef_intro (fheader_intro rt fid la) lb) 
+                                          (block_intro l' ps' cs' tmn') cs' tmn' (initLocals la (params2GVs TD lp lc gl)) 
+                                          (params2GVs TD lp lc gl) nil)::
+                                        (mkEC F B ((insn_call rid noret0 tailc0 rt fid lp)::cs) tmn lc arg0 als)::EC) gl Mem0),
+                    trace_nil)
+            end
+          else None
+        else None
+      end
+    end
+  end
+end.
+
+Lemma dsInsn__implies__interInsn : forall state state' tr,
+  dsInsn state state' tr ->
+  interInsn state = Some (state', tr).
+Proof. 
+  intros state state' tr HdsInsn.
+  (dsInsn_cases (destruct HdsInsn) Case); simpl;
+    try solve [rewrite H; simpl; rewrite H0; simpl; rewrite H1; simpl; auto |
+               rewrite H; simpl; rewrite H0; simpl; auto |
+               rewrite H; simpl; auto ].
+  Case "dsBranch".
+    rewrite H. simpl. rewrite <- H0. simpl. auto.
+  Case "dsBranch_uncond".
+    rewrite <- H. simpl. auto.
+  Case "dsCall".
+    rewrite H. simpl in H0. rewrite H0. 
+    destruct (id_dec fid fid); auto.
+      destruct (typ_dec rt rt); auto.
+        contradict n; auto.
+      contradict n; auto.
+Qed.
+
+Lemma interInsn__implies__dsInsn : forall state state' tr,
+  interInsn state = Some (state', tr) ->
+  dsInsn state state' tr.
+Proof.
+  intros state state' tr HinterInsn.
+  destruct state.
+  destruct ECS0; simpl in HinterInsn;
+    try solve [inversion HinterInsn].
+
+    destruct e as [F B cs tmn lc arg0 als].
+    destruct cs.
+      destruct tmn.
+      Case "insn_return".
+        destruct ECS0;
+          try solve [inversion HinterInsn].
+          
+          destruct e as [F' B' cs' tmn' lc' arg' als'].
+          destruct cs';
+            try solve [inversion HinterInsn].
+
+            remember (Instruction.isCallInst c) as R1.
+            remember (free_allocas Mem0 als) as R2.
+            destruct R1; try solve [inversion HinterInsn].
+            destruct R2; inversion HinterInsn; subst; eauto.
+
+      Case "insn_return_void".
+        destruct ECS0;
+          try solve [inversion HinterInsn].
+          
+          destruct e as [F' B' cs' tmn' lc' arg' als'].
+          destruct cs';
+            try solve [inversion HinterInsn].
+
+            remember (Instruction.isCallInst c) as R1.
+            remember (free_allocas Mem0 als) as R2.
+            destruct R1; try solve [inversion HinterInsn].
+            destruct R2; inversion HinterInsn; subst; eauto.
+
+      Case "insn_br".
+        remember (getOperandInt CurTargetData0 1 v lc Globals0) as R1.
+        destruct R1; try solve [inversion HinterInsn].
+          simpl in HinterInsn.
+          destruct n.
+            remember (lookupBlockViaLabelFromFdef F l0) as R2.
+            destruct R2; inversion HinterInsn; subst.
+              destruct b.
+              inversion HinterInsn; subst; eauto.
+        
+            remember (lookupBlockViaLabelFromFdef F l1) as R2.
+            destruct R2; inversion HinterInsn; subst.
+              destruct b.
+              inversion HinterInsn; subst; eauto.
+
+      Case "insn_br_uncond".
+        remember (lookupBlockViaLabelFromFdef F l0) as R2.
+        destruct R2; inversion HinterInsn; subst.
+          destruct b.
+          inversion HinterInsn; subst; eauto.
+
+      Case "insn_unreachable".
+        inversion HinterInsn.
+                    
+      destruct c.
+      Case "insn_bop".
+        remember (BOP CurTargetData0 lc Globals0 b s v v0) as R1.
+        destruct R1; 
+          simpl in HinterInsn;
+          inversion HinterInsn; subst; eauto.
+          
+      Case "insn_extractvalue".
+        remember (getOperandValue CurTargetData0 v lc Globals0) as R1.
+        destruct R1; simpl in HinterInsn; 
+          try solve [inversion HinterInsn].         
+        remember (extractGenericValue CurTargetData0 t g l0) as R2.
+        destruct R2; simpl in HinterInsn; 
+          inversion HinterInsn; subst; eauto.
+
+      Case "insn_insertvalue".
+        remember (getOperandValue CurTargetData0 v lc Globals0) as R1.
+        destruct R1; simpl in HinterInsn; 
+          try solve [inversion HinterInsn].         
+        remember (getOperandValue CurTargetData0 v0 lc Globals0) as R2.
+        destruct R2; simpl in HinterInsn; 
+          try solve [inversion HinterInsn].         
+        remember (insertGenericValue CurTargetData0 t g l0 t0 g0) as R3.
+        destruct R3; simpl in HinterInsn; 
+          inversion HinterInsn; subst; eauto.
+          
+      Case "insn_malloc".
+        remember (getTypeAllocSize CurTargetData0 t) as R1.
+        destruct R1; simpl in HinterInsn; 
+          try solve [inversion HinterInsn].         
+        remember (malloc CurTargetData0 Mem0 (n*s) a) as R2.
+        destruct R2; simpl in HinterInsn; 
+          try solve [inversion HinterInsn].         
+        destruct p; 
+          inversion HinterInsn; subst; eauto.
+          
+      Case "insn_free".
+        remember (getOperandPtr CurTargetData0 v lc Globals0) as R1.
+        destruct R1; simpl in HinterInsn; 
+          try solve [inversion HinterInsn].         
+        remember (free Mem0 m) as R2.
+        destruct R2; simpl in HinterInsn; 
+          inversion HinterInsn; subst; eauto.
+          
+      Case "insn_alloca".
+        remember (getTypeAllocSize CurTargetData0 t) as R1.
+        destruct R1; simpl in HinterInsn; 
+          try solve [inversion HinterInsn].         
+        remember (malloc CurTargetData0 Mem0 (n*s) a) as R2.
+        destruct R2; simpl in HinterInsn; 
+          try solve [inversion HinterInsn].         
+        destruct p; 
+          inversion HinterInsn; subst; eauto.
+          
+      Case "insn_load".
+        remember (getOperandPtr CurTargetData0 v lc Globals0) as R1.
+        destruct R1; simpl in HinterInsn; 
+          try solve [inversion HinterInsn].         
+        remember (mload CurTargetData0 Mem0 m t a) as R2.
+        destruct R2; simpl in HinterInsn; 
+          inversion HinterInsn; subst; eauto.
+          
+      Case "insn_store".
+        remember (getOperandValue CurTargetData0 v lc Globals0) as R1.
+        destruct R1; simpl in HinterInsn; 
+          try solve [inversion HinterInsn].         
+        remember (getOperandPtr CurTargetData0 v0 lc Globals0) as R2.
+        destruct R2; simpl in HinterInsn; 
+          try solve [inversion HinterInsn].         
+        remember (mstore CurTargetData0 Mem0 m t g a) as R3.
+        destruct R3; simpl in HinterInsn; 
+          inversion HinterInsn; subst; eauto.
+          
+      Case "insn_gep".
+        remember (getOperandPtr CurTargetData0 v lc Globals0) as R1.
+        destruct R1; simpl in HinterInsn; 
+          try solve [inversion HinterInsn].         
+        remember (GEP CurTargetData0 lc Globals0 t m l0 i1) as R2.
+        destruct R2; simpl in HinterInsn; 
+          inversion HinterInsn; subst; eauto.
+
+      Case "insn_ext".
+        remember (EXT CurTargetData0 lc Globals0 e t v t0) as R.
+        destruct R; simpl in HinterInsn; 
+          inversion HinterInsn; subst; eauto.
+
+      Case "insn_cast".
+        remember (CAST CurTargetData0 lc Globals0 c t v t0) as R.
+        destruct R; simpl in HinterInsn; 
+          inversion HinterInsn; subst; eauto.
+
+      Case "insn_icmp".
+        remember (ICMP CurTargetData0 lc Globals0 c t v v0) as R.
+        destruct R; simpl in HinterInsn; 
+          inversion HinterInsn; subst; eauto.
+
+      Case "insn_select".
+        remember (getOperandInt CurTargetData0 1 v lc Globals0) as R1.
+        destruct R1; simpl in HinterInsn; 
+          try solve [inversion HinterInsn].         
+        remember (getOperandValue CurTargetData0 v0 lc Globals0) as R2.
+        destruct R2; simpl in HinterInsn; 
+          try solve [inversion HinterInsn].         
+        remember (getOperandValue CurTargetData0 v1 lc Globals0) as R3.
+        destruct R3; simpl in HinterInsn; 
+          try solve [inversion HinterInsn].
+        inversion HinterInsn; subst; eauto.
+
+      Case "insn_call".
+        remember (lookupFdefViaIDFromProducts CurProducts0 i1) as R1.
+        destruct R1; simpl in HinterInsn; 
+          try solve [inversion HinterInsn].
+        destruct f. destruct f.
+        destruct (id_dec i1 i2); try solve [inversion HinterInsn]; subst.
+        destruct (typ_dec t0 t1); try solve [inversion HinterInsn]; subst.
+        destruct b; try solve [inversion HinterInsn].
+        destruct b.
+        inversion HinterInsn; subst; eauto.
+Qed.
+
+Extraction interInsn.
+
+
